share/steel/examples/pulse/parallel/GhostTaskQueue.fsti
@@ -74,12 +74,20 @@ stt_atomic (pos:nat & certificate r (pop_todo_task l)._1 pos) #Unobservable (sin
 (M.pts_to r one_half l)
 (fun _ -> M.pts_to r one_half (pop_todo_task l)._2 ** ongoing_condition (pop_todo_task l)._1 ** GR.pts_to (pop_todo_task l)._1._1 #one_half true ** GR.pts_to (pop_todo_task l)._1._2 #one_half false)
 
+(*
+the `task_done t` in the postcondition is actually not needed, because it's the worker that calls this function
+*)
 val conclude_task (t: task) (pos: nat) (r: ghost_mono_ref) (i: inv (inv_ghost_queue r)) (l: mono_list{task_in_queue t pos l}):
 stt_atomic unit (singleton i)
 (M.pts_to r one_half l ** GR.pts_to t._1 #one_half false ** GR.pts_to t._2 #one_half true ** ongoing_condition t ** (exists* v. pts_to t._4._1 #one_half v))
 (fun () -> M.pts_to r one_half (close_task_bis t pos l) ** pts_to t._4._1 #one_half true ** task_done t)
 
-val get_free_task_done (t: task) (pos: nat) (r: ghost_mono_ref) (i: inv (inv_ghost_queue r)) (l: mono_list{task_in_queue t pos l}):
-stt_atomic unit (singleton i)
-(M.pts_to r one_half l)
-(fun () -> M.pts_to r one_half l ** task_done t)
+val get_free_task_done (t: task) (pos: nat) (r: ghost_mono_ref) (i: inv (inv_ghost_queue r)) (ll: mono_list{task_in_queue t pos ll}):
+stt_atomic unit #Unobservable (singleton i)
+(M.pts_to r one_half ll ** pure (get_actual_queue ll == [] /\ count_ongoing ll = 0))
+(fun () -> M.pts_to r one_half ll ** task_done t)
+
+val get_task_in_queue (r: ghost_mono_ref) (f: perm) (l: mono_list) (t: task) (pos: nat) (w: certificate r t pos):
+stt_atomic unit #Unobservable emp_inames
+(M.pts_to r f l)
+(fun () -> M.pts_to r f l ** pure (task_in_queue t pos l))
